\documentclass[a4paper, draft]{article}
\usepackage[utf8]{inputenc}
\usepackage[australian]{babel}
\usepackage{mathtools}
\title{Preliminary 3 Unit Notes}
\author{Curly Macadam}
\date{}
\begin{document}
\maketitle
\section{Algebra}
\subsection{Index laws}
\begin{enumerate}
\item \(a^m \times a^n = a^{m+n}\)
\item \(a^m \div a^n = a^{m-n}\)
\item \((a^m)^n = a^{mn}\)
\item \((ab)^n = a^{n}b^{n}\)
\item \(\left(\dfrac{a}{b}\right)^n = \dfrac{a^n}{b^n}\)
\item \(a^0 = 1\)
\item \(a^{-n} = \dfrac{1}{x^n}\)
\item \(a^{\frac{1}{n}} = \sqrt[n]{a}\)
\end{enumerate}
\subsection{Binomial Products}
\[\begin{align*}
(a+b)(x+y) &= ax + ay + bx + by \\
(a+b)(a-b) &= a^2 - b^2 \\
(a+b)^2 &= a^2 + 2ab + b^2 \\
(a-b)^2 &= a^2 - 2ab + b^2
\end{align*}\]
\subsection{Factorising}
\[\begin{align*}
x^2 + (a+b) + ab &= (x+a)(x+b) \\
a^3 + b^3 &= (a+b)(a^2 - ab + b^2) \\
a^3 - b^3 &= (a-b)(a^2 + ab + b^2)
\end{align*}
\]
\end{document}
